Remove context reduction from pred1_extra

pcuic/theories/PCUICPredExtra.v
@@ -32,454 +32,518 @@ Section ParallelReductionExtra.
   (* Potential extra rules, might be redundant *)
   Context (extra : option (kername × rewrite_decl)).
 
-  Inductive pred1_extra (Γ Γ' : context) : term -> term -> Type :=
+  Inductive pred1_extra (Γ : context) : term -> term -> Type :=
   (** Reductions *)
   (** Beta *)
   | predx_beta na t0 t1 b0 b1 a0 a1 :
-      pred1_extra Γ Γ' t0 t1 ->
-      pred1_extra (Γ ,, vass na t0) (Γ' ,, vass na t1) b0 b1 -> pred1_extra Γ Γ' a0 a1 ->
-      pred1_extra Γ Γ' (tApp (tLambda na t0 b0) a0) (subst10 a1 b1)
+      pred1_extra Γ t0 t1 ->
+      pred1_extra (Γ ,, vass na t0) b0 b1 ->
+      pred1_extra Γ a0 a1 ->
+      pred1_extra Γ (tApp (tLambda na t0 b0) a0) (subst10 a1 b1)
 
   (** Let *)
   | predx_zeta na d0 d1 t0 t1 b0 b1 :
-      pred1_extra Γ Γ' t0 t1 ->
-      pred1_extra Γ Γ' d0 d1 -> pred1_extra (Γ ,, vdef na d0 t0) (Γ' ,, vdef na d1 t1) b0 b1 ->
-      pred1_extra Γ Γ' (tLetIn na d0 t0 b0) (subst10 d1 b1)
+      pred1_extra Γ t0 t1 ->
+      pred1_extra Γ d0 d1 ->
+      pred1_extra (Γ ,, vdef na d0 t0) b0 b1 ->
+      pred1_extra Γ (tLetIn na d0 t0 b0) (subst10 d1 b1)
 
   (** Local variables *)
   | predx_rel_def_unfold i body :
-      All2_local_env (on_decl pred1_extra) Γ Γ' ->
-      option_map decl_body (nth_error Γ' i) = Some (Some body) ->
-      pred1_extra Γ Γ' (tRel i) (lift0 (S i) body)
+      option_map decl_body (nth_error Γ i) = Some (Some body) ->
+      pred1_extra Γ (tRel i) (lift0 (S i) body)
 
   | predx_rel_refl i :
-      All2_local_env (on_decl pred1_extra) Γ Γ' ->
-      pred1_extra Γ Γ' (tRel i)  (tRel i)
+      pred1_extra Γ (tRel i)  (tRel i)
 
   (** Case *)
   | predx_iota ind pars c u args0 args1 p brs0 brs1 :
-      All2_local_env (on_decl pred1_extra) Γ Γ' ->
-      All2 (pred1_extra Γ Γ') args0 args1 ->
-      All2 (on_Trel_eq (pred1_extra Γ Γ') snd fst) brs0 brs1 ->
-      pred1_extra Γ Γ' (tCase (ind, pars) p (mkApps (tConstruct ind c u) args0) brs0)
-            (iota_red pars c args1 brs1)
+      All2 (pred1_extra Γ) args0 args1 ->
+      All2 (on_Trel_eq (pred1_extra Γ) snd fst) brs0 brs1 ->
+      pred1_extra Γ (tCase (ind, pars) p
+        (mkApps (tConstruct ind c u) args0) brs0)
+        (iota_red pars c args1 brs1)
 
   (** Fix unfolding, with guard *)
   | predx_fix mfix0 mfix1 idx args0 args1 narg fn :
-      All2_local_env (on_decl pred1_extra) Γ Γ' ->
-      All2_local_env (on_decl (on_decl_over pred1_extra Γ Γ')) (fix_context mfix0) (fix_context mfix1) ->
-      All2_prop2_eq Γ Γ' (Γ ,,, fix_context mfix0) (Γ' ,,, fix_context mfix1)
-                    dtype dbody (fun x => (dname x, rarg x)) pred1_extra mfix0 mfix1 ->
+      All2 (fun x y =>
+        pred1_extra Γ x.(dtype) y.(dtype) ×
+        pred1_extra (Γ ,,, fix_context mfix0) x.(dbody) y.(dbody) ×
+        x.(rarg) = y.(rarg)
+      ) mfix0 mfix1 ->
       unfold_fix mfix1 idx = Some (narg, fn) ->
       is_constructor narg args0 = true ->
-      All2 (pred1_extra Γ Γ') args0 args1 ->
-      pred1_extra Γ Γ' (mkApps (tFix mfix0 idx) args0) (mkApps fn args1)
+      All2 (pred1_extra Γ) args0 args1 ->
+      pred1_extra Γ (mkApps (tFix mfix0 idx) args0) (mkApps fn args1)
 
   (** CoFix-case unfolding *)
   | predx_cofix_case ip p0 p1 mfix0 mfix1 idx args0 args1 narg fn brs0 brs1 :
-      All2_local_env (on_decl pred1_extra) Γ Γ' ->
-      All2_local_env (on_decl (on_decl_over pred1_extra Γ Γ')) (fix_context mfix0) (fix_context mfix1) ->
-      All2_prop2_eq Γ Γ' (Γ ,,, fix_context mfix0) (Γ' ,,, fix_context mfix1)
-                    dtype dbody (fun x => (dname x, rarg x)) pred1_extra mfix0 mfix1 ->
+      All2 (fun x y =>
+        pred1_extra Γ x.(dtype) y.(dtype) ×
+        pred1_extra (Γ ,,, fix_context mfix0) x.(dbody) y.(dbody) ×
+        x.(rarg) = y.(rarg)
+      ) mfix0 mfix1 ->
       unfold_cofix mfix1 idx = Some (narg, fn) ->
-      All2 (pred1_extra Γ Γ') args0 args1 ->
-      pred1_extra Γ Γ' p0 p1 ->
-      All2 (on_Trel_eq (pred1_extra Γ Γ') snd fst) brs0 brs1 ->
-      pred1_extra Γ Γ' (tCase ip p0 (mkApps (tCoFix mfix0 idx) args0) brs0)
-            (tCase ip p1 (mkApps fn args1) brs1)
+      All2 (pred1_extra Γ) args0 args1 ->
+      pred1_extra Γ p0 p1 ->
+      All2 (on_Trel_eq (pred1_extra Γ) snd fst) brs0 brs1 ->
+      pred1_extra Γ
+        (tCase ip p0 (mkApps (tCoFix mfix0 idx) args0) brs0)
+        (tCase ip p1 (mkApps fn args1) brs1)
 
   (** CoFix-proj unfolding *)
   | predx_cofix_proj p mfix0 mfix1 idx args0 args1 narg fn :
-      All2_local_env (on_decl pred1_extra) Γ Γ' ->
-      All2_local_env (on_decl (on_decl_over pred1_extra Γ Γ')) (fix_context mfix0) (fix_context mfix1) ->
-      All2_prop2_eq Γ Γ' (Γ ,,, fix_context mfix0) (Γ' ,,, fix_context mfix1)
-                    dtype dbody (fun x => (dname x, rarg x)) pred1_extra mfix0 mfix1 ->
+      All2 (fun x y =>
+        pred1_extra Γ x.(dtype) y.(dtype) ×
+        pred1_extra (Γ ,,, fix_context mfix0) x.(dbody) y.(dbody) ×
+        x.(rarg) = y.(rarg)
+      ) mfix0 mfix1 ->
       unfold_cofix mfix1 idx = Some (narg, fn) ->
-      All2 (pred1_extra Γ Γ') args0 args1 ->
-      pred1_extra Γ Γ' (tProj p (mkApps (tCoFix mfix0 idx) args0))
-            (tProj p (mkApps fn args1))
+      All2 (pred1_extra Γ) args0 args1 ->
+      pred1_extra Γ
+        (tProj p (mkApps (tCoFix mfix0 idx) args0))
+        (tProj p (mkApps fn args1))
 
   (** Symbols and rewrite rules  *)
 
   | predx_symb k n u :
-      All2_local_env (on_decl pred1_extra) Γ Γ' ->
-      pred1_extra Γ Γ' (tSymb k n u) (tSymb k n u)
+      pred1_extra Γ (tSymb k n u) (tSymb k n u)
 
   | predx_rewrite_rule k ui decl n r s s' :
-      All2_local_env (on_decl pred1_extra) Γ Γ' ->
       declared_symbol Σ k decl ->
       nth_error decl.(rules) n = Some r ->
-      All2 (pred1_extra Γ Γ') s s' ->
+      All2 (pred1_extra Γ) s s' ->
       let ss := symbols_subst k 0 ui #|decl.(symbols)| in
       untyped_subslet Γ s (subst_context ss 0 r.(pat_context)) ->
       let lhs := subst0 s (subst ss #|s| (lhs r)) in
       let rhs := subst0 s' (subst ss #|s| (rhs r)) in
-      pred1_extra Γ Γ' lhs rhs
+      pred1_extra Γ lhs rhs
 
   | predx_par_rewrite_rule k ui decl n r s s' :
-      All2_local_env (on_decl pred1_extra) Γ Γ' ->
       declared_symbol Σ k decl ->
       nth_error decl.(prules) n = Some r ->
-      All2 (pred1_extra Γ Γ') s s' ->
+      All2 (pred1_extra Γ) s s' ->
       let ss := symbols_subst k 0 ui #|decl.(symbols)| in
       untyped_subslet Γ s (subst_context ss 0 r.(pat_context)) ->
       let lhs := subst0 s (subst ss #|s| (lhs r)) in
       let rhs := subst0 s' (subst ss #|s| (rhs r)) in
-      pred1_extra Γ Γ' lhs rhs
+      pred1_extra Γ lhs rhs
 
   | predx_extra_rewrite_rule k ui decl n r s s' :
-      All2_local_env (on_decl pred1_extra) Γ Γ' ->
       extra = Some (k, decl) →
       nth_error (all_rewrite_rules decl) n = Some r ->
-      All2 (pred1_extra Γ Γ') s s' ->
+      All2 (pred1_extra Γ) s s' ->
       let ss := symbols_subst k 0 ui #|decl.(symbols)| in
       untyped_subslet Γ s (subst_context ss 0 r.(pat_context)) ->
       let lhs := subst0 s (subst ss #|s| (lhs r)) in
       let rhs := subst0 s' (subst ss #|s| (rhs r)) in
-      pred1_extra Γ Γ' lhs rhs
+      pred1_extra Γ lhs rhs
 
   (** Constant unfolding *)
 
   | predx_delta c decl body (isdecl : declared_constant Σ c decl) u :
-      All2_local_env (on_decl pred1_extra) Γ Γ' ->
       decl.(cst_body) = Some body ->
-      pred1_extra Γ Γ' (tConst c u) (subst_instance_constr u body)
+      pred1_extra Γ (tConst c u) (subst_instance_constr u body)
 
   | predx_const c u :
-      All2_local_env (on_decl pred1_extra) Γ Γ' ->
-      pred1_extra Γ Γ' (tConst c u) (tConst c u)
+      pred1_extra Γ (tConst c u) (tConst c u)
 
   (** Proj *)
   | predx_proj i pars narg k u args0 args1 arg1 :
-      All2_local_env (on_decl pred1_extra) Γ Γ' ->
-      All2 (pred1_extra Γ Γ') args0 args1 ->
+      All2 (pred1_extra Γ) args0 args1 ->
       nth_error args1 (pars + narg) = Some arg1 ->
-      pred1_extra Γ Γ' (tProj (i, pars, narg) (mkApps (tConstruct i k u) args0)) arg1
+      pred1_extra Γ
+        (tProj (i, pars, narg) (mkApps (tConstruct i k u) args0))
+        arg1
 
   (** Congruences *)
-  | predx_abs na M M' N N' : pred1_extra Γ Γ' M M' -> pred1_extra (Γ ,, vass na M) (Γ' ,, vass na M') N N' ->
-                            pred1_extra Γ Γ' (tLambda na M N) (tLambda na M' N')
+  | predx_abs na M M' N N' :
+      pred1_extra Γ M M' ->
+      pred1_extra (Γ ,, vass na M) N N' ->
+      pred1_extra Γ (tLambda na M N) (tLambda na M' N')
+
   | predx_app M0 M1 N0 N1 :
-      pred1_extra Γ Γ' M0 M1 ->
-      pred1_extra Γ Γ' N0 N1 ->
-      pred1_extra Γ Γ' (tApp M0 N0) (tApp M1 N1)
-            (* do not handle mkApps yet *)
+      pred1_extra Γ M0 M1 ->
+      pred1_extra Γ N0 N1 ->
+      pred1_extra Γ (tApp M0 N0) (tApp M1 N1)
 
   | predx_letin na d0 d1 t0 t1 b0 b1 :
-      pred1_extra Γ Γ' d0 d1 -> pred1_extra Γ Γ' t0 t1 -> pred1_extra (Γ ,, vdef na d0 t0) (Γ' ,, vdef na d1 t1) b0 b1 ->
-      pred1_extra Γ Γ' (tLetIn na d0 t0 b0) (tLetIn na d1 t1 b1)
+      pred1_extra Γ  d0 d1 ->
+      pred1_extra Γ t0 t1 ->
+      pred1_extra (Γ ,, vdef na d0 t0) b0 b1 ->
+      pred1_extra Γ (tLetIn na d0 t0 b0) (tLetIn na d1 t1 b1)
 
   | predx_case ind p0 p1 c0 c1 brs0 brs1 :
-      pred1_extra Γ Γ' p0 p1 ->
-      pred1_extra Γ Γ' c0 c1 ->
-      All2 (on_Trel_eq (pred1_extra Γ Γ') snd fst) brs0 brs1 ->
-      pred1_extra Γ Γ' (tCase ind p0 c0 brs0) (tCase ind p1 c1 brs1)
+      pred1_extra Γ p0 p1 ->
+      pred1_extra Γ c0 c1 ->
+      All2 (on_Trel_eq (pred1_extra Γ) snd fst) brs0 brs1 ->
+      pred1_extra Γ (tCase ind p0 c0 brs0) (tCase ind p1 c1 brs1)
 
   | predx_proj_congr p c c' :
-      pred1_extra Γ Γ' c c' -> pred1_extra Γ Γ' (tProj p c) (tProj p c')
+      pred1_extra Γ c c' ->
+      pred1_extra Γ (tProj p c) (tProj p c')
 
   | predx_fix_congr mfix0 mfix1 idx :
-      All2_local_env (on_decl pred1_extra) Γ Γ' ->
-      All2_local_env (on_decl (on_decl_over pred1_extra Γ Γ')) (fix_context mfix0) (fix_context mfix1) ->
-      All2_prop2_eq Γ Γ' (Γ ,,, fix_context mfix0) (Γ' ,,, fix_context mfix1)
-                    dtype dbody (fun x => (dname x, rarg x)) pred1_extra mfix0 mfix1 ->
-      pred1_extra Γ Γ' (tFix mfix0 idx) (tFix mfix1 idx)
+      All2 (fun x y =>
+        pred1_extra Γ x.(dtype) y.(dtype) ×
+        pred1_extra (Γ ,,, fix_context mfix0) x.(dbody) y.(dbody) ×
+        x.(rarg) = y.(rarg)
+      ) mfix0 mfix1 ->
+      pred1_extra Γ (tFix mfix0 idx) (tFix mfix1 idx)
 
   | predx_cofix_congr mfix0 mfix1 idx :
-      All2_local_env (on_decl pred1_extra) Γ Γ' ->
-      All2_local_env (on_decl (on_decl_over pred1_extra Γ Γ')) (fix_context mfix0) (fix_context mfix1) ->
-      All2_prop2_eq Γ Γ' (Γ ,,, fix_context mfix0) (Γ' ,,, fix_context mfix1)
-                    dtype dbody (fun x => (dname x, rarg x)) pred1_extra mfix0 mfix1 ->
-      pred1_extra Γ Γ' (tCoFix mfix0 idx) (tCoFix mfix1 idx)
+      All2 (fun x y =>
+        pred1_extra Γ x.(dtype) y.(dtype) ×
+        pred1_extra (Γ ,,, fix_context mfix0) x.(dbody) y.(dbody) ×
+        x.(rarg) = y.(rarg)
+      ) mfix0 mfix1 ->
+      pred1_extra Γ (tCoFix mfix0 idx) (tCoFix mfix1 idx)
 
-  | predx_prod na M0 M1 N0 N1 : pred1_extra Γ Γ' M0 M1 -> pred1_extra (Γ ,, vass na M0) (Γ' ,, vass na M1) N0 N1 ->
-                               pred1_extra Γ Γ' (tProd na M0 N0) (tProd na M1 N1)
+  | predx_prod na M0 M1 N0 N1 :
+      pred1_extra Γ M0 M1 ->
+      pred1_extra (Γ ,, vass na M0) N0 N1 ->
+      pred1_extra Γ (tProd na M0 N0) (tProd na M1 N1)
 
   | evar_pred ev l l' :
-      All2_local_env (on_decl pred1_extra) Γ Γ' ->
-      All2 (pred1_extra Γ Γ') l l' -> pred1_extra Γ Γ' (tEvar ev l) (tEvar ev l')
+      All2 (pred1_extra Γ) l l' ->
+      pred1_extra Γ (tEvar ev l) (tEvar ev l')
 
   | predx_atom_refl t :
-      All2_local_env (on_decl pred1_extra) Γ Γ' ->
-      pred_atom t -> pred1_extra Γ Γ' t t.
+      pred_atom t ->
+      pred1_extra Γ t t.
+
+  Lemma All2_impl_def :
+    ∀ {A B} {P Q : A → B → Type} (l : list A) (l' : list B),
+      All2 P l l' →
+      (∀ x y, P x y → Q x y) →
+      All2 Q l l'.
+  Proof.
+    intros A B P Q l l' hl h.
+    induction hl. 1: constructor.
+    constructor.
+    - eapply h. assumption.
+    - assumption.
+  Defined.
 
   Lemma pred1_extra_ind_all_ctx :
-    forall (P : forall (Γ Γ' : context) (t t0 : term), Type)
-           (Pctx : forall (Γ Γ' : context), Type),
-      let P' Γ Γ' x y := ((pred1_extra Γ Γ' x y) * P Γ Γ' x y)%type in
-      (forall Γ Γ', All2_local_env (on_decl pred1_extra) Γ Γ' -> All2_local_env (on_decl P) Γ Γ' -> Pctx Γ Γ') ->
-      (forall (Γ Γ' : context) (na : name) (t0 t1 b0 b1 a0 a1 : term),
-          pred1_extra (Γ ,, vass na t0) (Γ' ,, vass na t1) b0 b1 -> P (Γ ,, vass na t0) (Γ' ,, vass na t1) b0 b1 ->
-          pred1_extra Γ Γ' t0 t1 -> P Γ Γ' t0 t1 ->
-          pred1_extra Γ Γ' a0 a1 -> P Γ Γ' a0 a1 -> P Γ Γ' (tApp (tLambda na t0 b0) a0) (b1 {0 := a1})) ->
-      (forall (Γ Γ' : context) (na : name) (d0 d1 t0 t1 b0 b1 : term),
-          pred1_extra Γ Γ' t0 t1 -> P Γ Γ' t0 t1 ->
-          pred1_extra Γ Γ' d0 d1 -> P Γ Γ' d0 d1 ->
-          pred1_extra (Γ ,, vdef na d0 t0) (Γ' ,, vdef na d1 t1) b0 b1 ->
-          P (Γ ,, vdef na d0 t0) (Γ' ,, vdef na d1 t1) b0 b1 -> P Γ Γ' (tLetIn na d0 t0 b0) (b1 {0 := d1})) ->
-      (forall (Γ Γ' : context) (i : nat) (body : term),
-          All2_local_env (on_decl pred1_extra) Γ Γ' ->
-          Pctx Γ Γ' ->
-          option_map decl_body (nth_error Γ' i) = Some (Some body) ->
-          P Γ Γ' (tRel i) (lift0 (S i) body)) ->
-      (forall (Γ Γ' : context) (i : nat),
-          All2_local_env (on_decl pred1_extra) Γ Γ' ->
-          Pctx Γ Γ' ->
-          P Γ Γ' (tRel i) (tRel i)) ->
-      (forall (Γ Γ' : context) (ind : inductive) (pars c : nat) (u : Instance.t) (args0 args1 : list term)
-              (p : term) (brs0 brs1 : list (nat * term)),
-          All2_local_env (on_decl pred1_extra) Γ Γ' ->
-          Pctx Γ Γ' ->
-          All2 (P' Γ Γ') args0 args1 ->
-          All2_prop_eq Γ Γ' snd fst P' brs0 brs1 ->
-          P Γ Γ' (tCase (ind, pars) p (mkApps (tConstruct ind c u) args0) brs0) (iota_red pars c args1 brs1)) ->
-      (forall (Γ Γ' : context) (mfix0 mfix1 : mfixpoint term) (idx : nat) (args0 args1 : list term) (narg : nat) (fn : term),
-          All2_local_env (on_decl pred1_extra) Γ Γ' ->
-          Pctx Γ Γ' ->
-          All2_local_env (on_decl (on_decl_over pred1_extra Γ Γ')) (fix_context mfix0) (fix_context mfix1) ->
-          All2_local_env (on_decl (on_decl_over P Γ Γ')) (fix_context mfix0) (fix_context mfix1) ->
-          All2_prop2_eq Γ Γ' (Γ ,,, fix_context mfix0) (Γ' ,,, fix_context mfix1) dtype dbody
-                        (fun x => (dname x, rarg x)) P' mfix0 mfix1 ->
+    forall (P : forall (Γ : context) (t t0 : term), Type)
+           (* (Pctx : forall (Γ : context), Type) *),
+      let P' Γ x y := ((pred1_extra Γ x y) × P Γ x y)%type in
+      (* (forall Γ, All2_local_env (on_decl pred1_extra) Γ Γ' -> All2_local_env (on_decl P) Γ Γ' -> Pctx Γ Γ') -> *)
+      (forall (Γ : context) (na : name) (t0 t1 b0 b1 a0 a1 : term),
+          pred1_extra (Γ ,, vass na t0) b0 b1 ->
+          P (Γ ,, vass na t0) b0 b1 ->
+          pred1_extra Γ t0 t1 -> P Γ t0 t1 ->
+          pred1_extra Γ a0 a1 -> P Γ a0 a1 ->
+          P Γ (tApp (tLambda na t0 b0) a0) (b1 {0 := a1})
+      ) ->
+      (forall (Γ : context) (na : name) (d0 d1 t0 t1 b0 b1 : term),
+          pred1_extra Γ t0 t1 -> P Γ t0 t1 ->
+          pred1_extra Γ d0 d1 -> P Γ d0 d1 ->
+          pred1_extra (Γ ,, vdef na d0 t0) b0 b1 ->
+          P (Γ ,, vdef na d0 t0) b0 b1 ->
+          P Γ (tLetIn na d0 t0 b0) (b1 {0 := d1})
+      ) ->
+      (forall (Γ : context) (i : nat) (body : term),
+          option_map decl_body (nth_error Γ i) = Some (Some body) ->
+          P Γ (tRel i) (lift0 (S i) body)
+      ) ->
+      (forall (Γ : context) (i : nat),
+          P Γ (tRel i) (tRel i)
+      ) ->
+      (forall (Γ : context) (ind : inductive) (pars c : nat) (u : Instance.t)
+        (args0 args1 : list term)
+        (p : term) (brs0 brs1 : list (nat * term)),
+          All2 (P' Γ) args0 args1 ->
+          All2 (on_Trel_eq (P' Γ) snd fst) brs0 brs1 ->
+          P Γ
+            (tCase (ind, pars) p (mkApps (tConstruct ind c u) args0) brs0)
+            (iota_red pars c args1 brs1)
+      ) ->
+      (forall (Γ : context) (mfix0 mfix1 : mfixpoint term) (idx : nat)
+        (args0 args1 : list term) (narg : nat) (fn : term),
+          All2 (fun x y =>
+            P' Γ x.(dtype) y.(dtype) ×
+            P' (Γ ,,, fix_context mfix0) x.(dbody) y.(dbody) ×
+            x.(rarg) = y.(rarg)
+          ) mfix0 mfix1 ->
           unfold_fix mfix1 idx = Some (narg, fn) ->
           is_constructor narg args0 = true ->
-          All2 (P' Γ Γ') args0 args1 ->
-          P Γ Γ' (mkApps (tFix mfix0 idx) args0) (mkApps fn args1)) ->
-      (forall (Γ Γ' : context) (ip : inductive * nat) (p0 p1 : term) (mfix0 mfix1 : mfixpoint term) (idx : nat)
-              (args0 args1 : list term) (narg : nat) (fn : term) (brs0 brs1 : list (nat * term)),
-          All2_local_env (on_decl pred1_extra) Γ Γ' ->
-          Pctx Γ Γ' ->
-          All2_local_env (on_decl (on_decl_over pred1_extra Γ Γ')) (fix_context mfix0) (fix_context mfix1) ->
-          All2_local_env (on_decl (on_decl_over P Γ Γ')) (fix_context mfix0) (fix_context mfix1) ->
-          All2_prop2_eq Γ Γ' (Γ ,,, fix_context mfix0) (Γ' ,,, fix_context mfix1) dtype dbody
-                        (fun x => (dname x, rarg x)) P' mfix0 mfix1 ->
+          All2 (P' Γ) args0 args1 ->
+          P Γ (mkApps (tFix mfix0 idx) args0) (mkApps fn args1)
+      ) ->
+      (forall (Γ : context) (ip : inductive * nat) (p0 p1 : term)
+        (mfix0 mfix1 : mfixpoint term) (idx : nat)
+        (args0 args1 : list term) (narg : nat) (fn : term)
+        (brs0 brs1 : list (nat * term)),
+          All2 (fun x y =>
+            P' Γ x.(dtype) y.(dtype) ×
+            P' (Γ ,,, fix_context mfix0) x.(dbody) y.(dbody) ×
+            x.(rarg) = y.(rarg)
+          ) mfix0 mfix1 ->
           unfold_cofix mfix1 idx = Some (narg, fn) ->
-          All2 (P' Γ Γ') args0 args1 ->
-          pred1_extra Γ Γ' p0 p1 ->
-          P Γ Γ' p0 p1 ->
-          All2_prop_eq Γ Γ' snd fst P' brs0 brs1 ->
-          P Γ Γ' (tCase ip p0 (mkApps (tCoFix mfix0 idx) args0) brs0) (tCase ip p1 (mkApps fn args1) brs1)) ->
-      (forall (Γ Γ' : context) (p : projection) (mfix0 mfix1 : mfixpoint term)
-         (idx : nat) (args0 args1 : list term)
-         (narg : nat) (fn : term),
-          All2_local_env (on_decl pred1_extra) Γ Γ' ->
-          Pctx Γ Γ' ->
-          All2_local_env (on_decl (on_decl_over pred1_extra Γ Γ')) (fix_context mfix0) (fix_context mfix1) ->
-          All2_local_env (on_decl (on_decl_over P Γ Γ')) (fix_context mfix0) (fix_context mfix1) ->
-          All2_prop2_eq Γ Γ' (Γ ,,, fix_context mfix0) (Γ' ,,, fix_context mfix1) dtype dbody
-                        (fun x => (dname x, rarg x)) P' mfix0 mfix1 ->
+          All2 (P' Γ) args0 args1 ->
+          pred1_extra Γ p0 p1 ->
+          P Γ p0 p1 ->
+          All2 (on_Trel_eq (P' Γ) snd fst) brs0 brs1 ->
+          P Γ
+            (tCase ip p0 (mkApps (tCoFix mfix0 idx) args0) brs0)
+            (tCase ip p1 (mkApps fn args1) brs1)
+      ) ->
+      (forall (Γ : context) (p : projection) (mfix0 mfix1 : mfixpoint term)
+        (idx : nat) (args0 args1 : list term)
+        (narg : nat) (fn : term),
+          All2 (fun x y =>
+            P' Γ x.(dtype) y.(dtype) ×
+            P' (Γ ,,, fix_context mfix0) x.(dbody) y.(dbody) ×
+            x.(rarg) = y.(rarg)
+          ) mfix0 mfix1 ->
           unfold_cofix mfix1 idx = Some (narg, fn) ->
-          All2 (P' Γ Γ') args0 args1 ->
-          P Γ Γ' (tProj p (mkApps (tCoFix mfix0 idx) args0)) (tProj p (mkApps fn args1))) ->
-      (forall (Γ Γ' : context) (c : kername) (n : nat) (u : Instance.t),
-          All2_local_env (on_decl pred1_extra) Γ Γ' ->
-          Pctx Γ Γ' ->
-          P Γ Γ' (tSymb c n u) (tSymb c n u)) ->
-      (forall (Γ Γ' : context) k ui decl n r s s',
-          All2_local_env (on_decl pred1_extra) Γ Γ' ->
-          Pctx Γ Γ' ->
+          All2 (P' Γ) args0 args1 ->
+          P Γ
+            (tProj p (mkApps (tCoFix mfix0 idx) args0))
+            (tProj p (mkApps fn args1))
+      ) ->
+      (forall (Γ : context) (c : kername) (n : nat) (u : Instance.t),
+          P Γ (tSymb c n u) (tSymb c n u)
+      ) ->
+      (forall (Γ : context) k ui decl n r s s',
           declared_symbol Σ k decl ->
           nth_error decl.(rules) n = Some r ->
-          All2 (P' Γ Γ') s s' ->
+          All2 (P' Γ) s s' ->
           let ss := symbols_subst k 0 ui #|decl.(symbols)| in
           untyped_subslet Γ s (subst_context ss 0 r.(pat_context)) ->
           let lhs := subst0 s (subst ss #|s| (lhs r)) in
           let rhs := subst0 s' (subst ss #|s| (rhs r)) in
-          P Γ Γ' lhs rhs
+          P Γ lhs rhs
       ) ->
-      (forall (Γ Γ' : context) k ui decl n r s s',
-          All2_local_env (on_decl pred1_extra) Γ Γ' ->
-          Pctx Γ Γ' ->
+      (forall (Γ : context) k ui decl n r s s',
           declared_symbol Σ k decl ->
           nth_error decl.(prules) n = Some r ->
-          All2 (P' Γ Γ') s s' ->
+          All2 (P' Γ) s s' ->
           let ss := symbols_subst k 0 ui #|decl.(symbols)| in
           untyped_subslet Γ s (subst_context ss 0 r.(pat_context)) ->
           let lhs := subst0 s (subst ss #|s| (lhs r)) in
           let rhs := subst0 s' (subst ss #|s| (rhs r)) in
-          P Γ Γ' lhs rhs
+          P Γ lhs rhs
       ) ->
-      (forall (Γ Γ' : context) k ui decl n r s s',
-          All2_local_env (on_decl pred1_extra) Γ Γ' ->
-          Pctx Γ Γ' ->
+      (forall (Γ : context) k ui decl n r s s',
           extra = Some (k, decl) →
           nth_error (all_rewrite_rules decl) n = Some r ->
-          All2 (P' Γ Γ') s s' ->
+          All2 (P' Γ) s s' ->
           let ss := symbols_subst k 0 ui #|decl.(symbols)| in
           untyped_subslet Γ s (subst_context ss 0 r.(pat_context)) ->
           let lhs := subst0 s (subst ss #|s| (lhs r)) in
           let rhs := subst0 s' (subst ss #|s| (rhs r)) in
-          P Γ Γ' lhs rhs
+          P Γ lhs rhs
       ) ->
-      (forall (Γ Γ' : context) (c : kername) (decl : constant_body) (body : term),
-          All2_local_env (on_decl pred1_extra) Γ Γ' ->
-          Pctx Γ Γ' ->
+      (forall (Γ : context) (c : kername) (decl : constant_body) (body : term),
           declared_constant Σ c decl ->
           forall u : Instance.t, cst_body decl = Some body ->
-                                        P Γ Γ' (tConst c u) (subst_instance_constr u body)) ->
-      (forall (Γ Γ' : context) c (u : Instance.t),
-          All2_local_env (on_decl pred1_extra) Γ Γ' ->
-          Pctx Γ Γ' ->
-          P Γ Γ' (tConst c u) (tConst c u)) ->
-      (forall (Γ Γ' : context) (i : inductive) (pars narg : nat) (k : nat) (u : Instance.t)
-              (args0 args1 : list term) (arg1 : term),
-          All2_local_env (on_decl pred1_extra) Γ Γ' ->
-          Pctx Γ Γ' ->
-          All2 (pred1_extra Γ Γ') args0 args1 ->
-          All2 (P Γ Γ') args0 args1 ->
+          P Γ (tConst c u) (subst_instance_constr u body)
+      ) ->
+      (forall (Γ : context) c (u : Instance.t),
+          P Γ (tConst c u) (tConst c u)
+      ) ->
+      (forall (Γ : context) (i : inductive) (pars narg : nat) (k : nat)
+        (u : Instance.t) (args0 args1 : list term) (arg1 : term),
+          All2 (pred1_extra Γ) args0 args1 ->
+          All2 (P Γ) args0 args1 ->
           nth_error args1 (pars + narg) = Some arg1 ->
-          P Γ Γ' (tProj (i, pars, narg) (mkApps (tConstruct i k u) args0)) arg1) ->
-      (forall (Γ Γ' : context) (na : name) (M M' N N' : term),
-          pred1_extra Γ Γ' M M' ->
-          P Γ Γ' M M' -> pred1_extra (Γ,, vass na M) (Γ' ,, vass na M') N N' ->
-          P (Γ,, vass na M) (Γ' ,, vass na M') N N' -> P Γ Γ' (tLambda na M N) (tLambda na M' N')) ->
-      (forall (Γ Γ' : context) (M0 M1 N0 N1 : term),
-          pred1_extra Γ Γ' M0 M1 -> P Γ Γ' M0 M1 -> pred1_extra Γ Γ' N0 N1 ->
-          P Γ Γ' N0 N1 -> P Γ Γ' (tApp M0 N0) (tApp M1 N1)) ->
-      (forall (Γ Γ' : context) (na : name) (d0 d1 t0 t1 b0 b1 : term),
-          pred1_extra Γ Γ' d0 d1 ->
-          P Γ Γ' d0 d1 ->
-          pred1_extra Γ Γ' t0 t1 ->
-          P Γ Γ' t0 t1 ->
-          pred1_extra (Γ,, vdef na d0 t0) (Γ',,vdef na d1 t1) b0 b1 ->
-          P (Γ,, vdef na d0 t0) (Γ',,vdef na d1 t1) b0 b1 -> P Γ Γ' (tLetIn na d0 t0 b0) (tLetIn na d1 t1 b1)) ->
-      (forall (Γ Γ' : context) (ind : inductive * nat) (p0 p1 c0 c1 : term) (brs0 brs1 : list (nat * term)),
-          pred1_extra Γ Γ' p0 p1 ->
-          P Γ Γ' p0 p1 ->
-          pred1_extra Γ Γ' c0 c1 ->
-          P Γ Γ' c0 c1 -> All2_prop_eq Γ Γ' snd fst P' brs0 brs1 ->
-          P Γ Γ' (tCase ind p0 c0 brs0) (tCase ind p1 c1 brs1)) ->
-      (forall (Γ Γ' : context) (p : projection) (c c' : term), pred1_extra Γ Γ' c c' -> P Γ Γ' c c' -> P Γ Γ' (tProj p c) (tProj p c')) ->
-
-      (forall (Γ Γ' : context) (mfix0 : mfixpoint term) (mfix1 : list (def term)) (idx : nat),
-          All2_local_env (on_decl pred1_extra) Γ Γ' ->
-          Pctx Γ Γ' ->
-          All2_local_env (on_decl (on_decl_over pred1_extra Γ Γ')) (fix_context mfix0) (fix_context mfix1) ->
-          All2_local_env (on_decl (on_decl_over P Γ Γ')) (fix_context mfix0) (fix_context mfix1) ->
-          All2_prop2_eq Γ Γ' (Γ ,,, fix_context mfix0) (Γ' ,,, fix_context mfix1)
-                        dtype dbody (fun x => (dname x, rarg x)) P' mfix0 mfix1 ->
-          P Γ Γ' (tFix mfix0 idx) (tFix mfix1 idx)) ->
-
-      (forall (Γ Γ' : context) (mfix0 : mfixpoint term) (mfix1 : list (def term)) (idx : nat),
-          All2_local_env (on_decl pred1_extra) Γ Γ' ->
-          Pctx Γ Γ' ->
-          All2_local_env (on_decl (on_decl_over pred1_extra Γ Γ')) (fix_context mfix0) (fix_context mfix1) ->
-          All2_local_env (on_decl (on_decl_over P Γ Γ')) (fix_context mfix0) (fix_context mfix1) ->
-          All2_prop2_eq Γ Γ' (Γ ,,, fix_context mfix0) (Γ' ,,, fix_context mfix1) dtype dbody (fun x => (dname x, rarg x)) P' mfix0 mfix1 ->
-          P Γ Γ' (tCoFix mfix0 idx) (tCoFix mfix1 idx)) ->
-      (forall (Γ Γ' : context) (na : name) (M0 M1 N0 N1 : term),
-          pred1_extra Γ Γ' M0 M1 ->
-          P Γ Γ' M0 M1 -> pred1_extra (Γ,, vass na M0) (Γ' ,, vass na M1) N0 N1 ->
-          P (Γ,, vass na M0) (Γ' ,, vass na M1) N0 N1 -> P Γ Γ' (tProd na M0 N0) (tProd na M1 N1)) ->
-      (forall (Γ Γ' : context) (ev : nat) (l l' : list term),
-          All2_local_env (on_decl pred1_extra) Γ Γ' ->
-          Pctx Γ Γ' ->
-          All2 (P' Γ Γ') l l' -> P Γ Γ' (tEvar ev l) (tEvar ev l')) ->
-      (forall (Γ Γ' : context) (t : term),
-          All2_local_env (on_decl pred1_extra) Γ Γ' ->
-          Pctx Γ Γ' ->
-          pred_atom t -> P Γ Γ' t t) ->
-      forall (Γ Γ' : context) (t t0 : term), pred1_extra Γ Γ' t t0 -> P Γ Γ' t t0.
+          P Γ (tProj (i, pars, narg) (mkApps (tConstruct i k u) args0)) arg1
+      ) ->
+      (forall (Γ : context) (na : name) (M M' N N' : term),
+          pred1_extra Γ M M' -> P Γ M M' ->
+          pred1_extra (Γ,, vass na M) N N' ->
+          P (Γ,, vass na M) N N' ->
+          P Γ (tLambda na M N) (tLambda na M' N')
+      ) ->
+      (forall (Γ : context) (M0 M1 N0 N1 : term),
+          pred1_extra Γ M0 M1 ->
+          P Γ M0 M1 ->
+          pred1_extra Γ N0 N1 ->
+          P Γ N0 N1 ->
+          P Γ (tApp M0 N0) (tApp M1 N1)
+      ) ->
+      (forall (Γ : context) (na : name) (d0 d1 t0 t1 b0 b1 : term),
+          pred1_extra Γ d0 d1 ->
+          P Γ d0 d1 ->
+          pred1_extra Γ t0 t1 ->
+          P Γ t0 t1 ->
+          pred1_extra (Γ,, vdef na d0 t0) b0 b1 ->
+          P (Γ,, vdef na d0 t0) b0 b1 ->
+          P Γ (tLetIn na d0 t0 b0) (tLetIn na d1 t1 b1)
+      ) ->
+      (forall (Γ : context) (ind : inductive * nat) (p0 p1 c0 c1 : term)
+        (brs0 brs1 : list (nat * term)),
+          pred1_extra Γ p0 p1 ->
+          P Γ p0 p1 ->
+          pred1_extra Γ c0 c1 ->
+          P Γ c0 c1 ->
+          All2 (on_Trel_eq (P' Γ) snd fst) brs0 brs1 ->
+          P Γ (tCase ind p0 c0 brs0) (tCase ind p1 c1 brs1)
+      ) ->
+      (forall (Γ : context) (p : projection) (c c' : term),
+          pred1_extra Γ c c' ->
+          P Γ c c' ->
+          P Γ (tProj p c) (tProj p c')
+      ) ->
+      (forall (Γ : context) (mfix0 : mfixpoint term) (mfix1 : list (def term))
+        (idx : nat),
+          All2 (fun x y =>
+            P' Γ x.(dtype) y.(dtype) ×
+            P' (Γ ,,, fix_context mfix0) x.(dbody) y.(dbody) ×
+            x.(rarg) = y.(rarg)
+          ) mfix0 mfix1 ->
+          P Γ (tFix mfix0 idx) (tFix mfix1 idx)
+      ) ->
+      (forall (Γ : context) (mfix0 : mfixpoint term) (mfix1 : list (def term))
+        (idx : nat),
+          All2 (fun x y =>
+            P' Γ x.(dtype) y.(dtype) ×
+            P' (Γ ,,, fix_context mfix0) x.(dbody) y.(dbody) ×
+            x.(rarg) = y.(rarg)
+          ) mfix0 mfix1 ->
+          P Γ (tCoFix mfix0 idx) (tCoFix mfix1 idx)
+      ) ->
+      (forall (Γ : context) (na : name) (M0 M1 N0 N1 : term),
+          pred1_extra Γ M0 M1 ->
+          P Γ M0 M1 ->
+          pred1_extra (Γ,, vass na M0) N0 N1 ->
+          P (Γ,, vass na M0) N0 N1 ->
+          P Γ (tProd na M0 N0) (tProd na M1 N1)
+      ) ->
+      (forall (Γ : context) (ev : nat) (l l' : list term),
+          All2 (P' Γ) l l' ->
+          P Γ (tEvar ev l) (tEvar ev l')
+      ) ->
+      (forall (Γ : context) (t : term),
+          pred_atom t ->
+          P Γ t t
+      ) ->
+      forall (Γ : context) (t t0 : term), pred1_extra Γ t t0 -> P Γ t t0.
   Proof.
-    intros P Pctx P' Hctx.
+    intros P P'.
     intros X X0 X1 X2 X3 X4 X5 X6 X7 Xrw Xprw Xxrw X8 X9 X10 X11 X12 X13 X14 X15 X16
-      X17 X18 X19 X20 Γ Γ' t t0 X21.
-    revert Γ Γ' t t0 X21.
-    fix aux 5. intros Γ Γ' t t'.
+      X17 X18 X19 X20 Γ t t0 X21.
+    revert Γ t t0 X21.
+    fix aux 4. intros Γ t t'.
     move aux at top.
     destruct 1; match goal with
-                | |- P _ _ (tFix _ _) (tFix _ _) => idtac
-                | |- P _ _ (tCoFix _ _) (tCoFix _ _) => idtac
-                | |- P _ _ (mkApps (tFix _ _) _) _ => idtac
-                | |- P _ _ (tCase _ _ (mkApps (tCoFix _ _) _) _) _ => idtac
-                | |- P _ _ (tProj _ (mkApps (tCoFix _ _) _)) _ => idtac
-                | |- P _ _ (tRel _) _ => idtac
-                | |- P _ _ (tSymb _ _ _) _ => idtac
-                | |- P _ _ (tConst _ _) _ => idtac
+                | |- P _ (tFix _ _) (tFix _ _) => idtac
+                | |- P _ (tCoFix _ _) (tCoFix _ _) => idtac
+                | |- P _ (mkApps (tFix _ _) _) _ => idtac
+                | |- P _ (tCase _ _ (mkApps (tCoFix _ _) _) _) _ => idtac
+                | |- P _ (tProj _ (mkApps (tCoFix _ _) _)) _ => idtac
+                | |- P _ (tRel _) _ => idtac
+                | |- P _ (tSymb _ _ _) _ => idtac
+                | |- P _ (tConst _ _) _ => idtac
                 | lhs := _, rhs := _ |- _ => idtac
                 | H : _ |- _ => eapply H; eauto
                 end.
-    - simpl. apply X1; auto. apply Hctx.
-      + apply (All2_local_env_impl a). intros. eapply X21.
-      + apply (All2_local_env_impl a). intros. eapply (aux _ _ _ _ X21).
-    - simpl. apply X2; auto.
-      apply Hctx, (All2_local_env_impl a).
-      + exact a.
-      + intros. apply (aux _ _ _ _ X21).
-    - apply Hctx, (All2_local_env_impl a). 1: exact a.
-      intros. apply (aux _ _ _ _ X21).
-    - eapply (All2_All2_prop (P:=pred1_extra) (Q:=P') a0 ((extendP aux) Γ Γ')).
-    - eapply (All2_All2_prop_eq (P:=pred1_extra) (Q:=P') (f:=snd) (g:=fst) a1 (extendP aux Γ Γ')).
-    - eapply X4; eauto.
-      + apply Hctx, (All2_local_env_impl a). 1: exact a.
-        intros. apply (aux _ _ _ _ X21).
-      + eapply (All2_local_env_impl a0). intros. red. red in X21.
-        apply (aux _ _ _ _ X21).
-      + eapply (All2_All2_prop2_eq (Q:=P') (f:=dtype) (g:=dbody) a1 (extendP aux)).
-      + eapply (All2_All2_prop (P:=pred1_extra) (Q:=P') a2 (extendP aux Γ Γ')).
-    - eapply X5; eauto.
-      + apply Hctx, (All2_local_env_impl a). 1: exact a.
-        intros. apply (aux _ _ _ _ X22).
-      + eapply (All2_local_env_impl a0). intros. red. red in X22.
-        apply (aux _ _ _ _ X22).
-      + eapply (All2_All2_prop2_eq (Q:=P') (f:=dtype) (g:=dbody) a1 (extendP aux)).
-      + eapply (All2_All2_prop (P:=pred1_extra) (Q:=P') a2 (extendP aux Γ Γ')).
-      + eapply (All2_All2_prop_eq (P:=pred1_extra) (Q:=P') (f:=snd) a3 (extendP aux Γ Γ')).
-    - eapply X6; eauto.
-      + apply Hctx, (All2_local_env_impl a). 1: exact a.
-        intros. apply (aux _ _ _ _ X21).
-      + eapply (All2_local_env_impl a0). intros. red. red in X21. apply (aux _ _ _ _ X21).
-      + eapply (All2_All2_prop2_eq (Q:=P') (f:=dtype) (g:=dbody) a1 (extendP aux)).
-      + eapply (All2_All2_prop (P:=pred1_extra) (Q:=P') a2 (extendP aux Γ Γ')).
-    - eapply X7. 1: assumption.
-      apply Hctx, (All2_local_env_impl a).
-      + intros. exact a.
-      + intros. apply (aux _ _ _ _ X21).
+    - apply X1. auto.
+    - apply X2.
+    - eapply All2_impl_def. 1: exact a.
+      intros. split. 1: auto.
+      apply (aux _ _ _ X21).
+    - eapply All2_impl_def. 1: eauto.
+      intros [? ?] [? ?]. cbn. intros [? ?].
+      split. 2: auto.
+      split. 1: auto.
+      eapply aux. auto.
+    - eapply X4. all: eauto.
+      + eapply All2_impl_def. 1: eauto.
+        intros [? ? ?] [? ? ?]. cbn. intros [? [? ?]].
+        intuition eauto.
+        * split. 1: auto.
+          eapply aux. auto.
+        * split. 1: auto.
+          eapply aux. auto.
+      + eapply All2_impl_def. 1: eauto.
+        intros. split. 1: auto.
+        eapply aux. auto.
+    - eapply X5. all: eauto.
+      + eapply All2_impl_def. 1: eauto.
+        intros [? ? ?] [? ? ?]. cbn. intros [? [? ?]].
+        intuition eauto.
+        * split. 1: auto.
+          eapply aux. auto.
+        * split. 1: auto.
+          eapply aux. auto.
+      + eapply All2_impl_def. 1: eauto.
+        intros. split. 1: auto.
+        eapply aux. auto.
+      + eapply All2_impl_def. 1: eauto.
+        intros [] []. cbn. intros [].
+        intuition auto.
+        split. 1: auto.
+        eapply aux. auto.
+    - eapply X6. all: eauto.
+      + eapply All2_impl_def. 1: eauto.
+        intros [? ? ?] [? ? ?]. cbn. intros [? [? ?]].
+        intuition auto.
+        * split. 1: auto.
+          eapply aux. auto.
+        * split. 1: auto.
+          eapply aux. auto.
+      + eapply All2_impl_def. 1: eauto.
+        intros. split. 1: auto.
+        eapply aux. auto.
+    - eapply X7.
     - eapply Xrw. all: eauto.
-      + apply Hctx. 1: auto.
-        apply (All2_local_env_impl a). intros. apply (aux _ _ _ _ X21).
-      + eapply (All2_All2_prop (P:=pred1_extra) (Q:=P') a0 ((extendP aux) Γ Γ')).
+      eapply All2_impl_def. 1: eauto.
+      intros. split. 1: auto.
+      eapply aux. auto.
     - eapply Xprw. all: eauto.
-      + apply Hctx. 1: auto.
-        apply (All2_local_env_impl a). intros. apply (aux _ _ _ _ X21).
-      + eapply (All2_All2_prop (P:=pred1_extra) (Q:=P') a0 ((extendP aux) Γ Γ')).
+      eapply All2_impl_def. 1: eauto.
+      intros. split. 1: auto.
+      eapply aux. auto.
     - eapply Xxrw. all: eauto.
-      + apply Hctx. 1: auto.
-        apply (All2_local_env_impl a). intros. apply (aux _ _ _ _ X21).
-      + eapply (All2_All2_prop (P:=pred1_extra) (Q:=P') a0 ((extendP aux) Γ Γ')).
-    - eapply X8; eauto.
-      apply Hctx, (All2_local_env_impl a).
-      + intros. exact a.
-      + intros. apply (aux _ _ _ _ X21).
+      eapply All2_impl_def. 1: eauto.
+      intros. split. 1: auto.
+      eapply aux. auto.
+    - eapply X8. all: eauto.
     - eapply X9; eauto.
-      apply Hctx, (All2_local_env_impl a). 1: exact a.
-      intros. apply (aux _ _ _ _ X21).
-    - apply Hctx, (All2_local_env_impl a). 1: exact a.
-      intros. apply (aux _ _ _ _ X21).
-    - eapply (All2_All2_prop (P:=pred1_extra) (Q:=P) a0). intros. apply (aux _ _ _ _ X21).
-    - eapply (All2_All2_prop_eq (P:=pred1_extra) (Q:=P') (f:=snd) a (extendP aux Γ Γ')).
+    - eapply All2_impl_def. 1: eauto.
+      intros.
+      eapply aux. auto.
+    - eapply All2_impl_def. 1: eauto.
+      intros [] []. cbn. intros [].
+      split. 2: auto.
+      split. 1: auto.
+      eapply aux. auto.
     - eapply X16.
-      + eapply (All2_local_env_impl a). intros. apply X21.
-      + eapply (Hctx _ _ a), (All2_local_env_impl a). intros. apply (aux _ _ _ _ X21).
-      + eapply (All2_local_env_impl a0). intros. red. exact X21.
-      + eapply (All2_local_env_impl a0). intros. red. apply (aux _ _ _ _ X21).
-      + eapply (All2_All2_prop2_eq (Q:=P') (f:=dtype) (g:=dbody) a1 (extendP aux)).
+      eapply All2_impl_def. 1: eauto.
+      intros [] []. cbn. intros [? [? ?]].
+      intuition auto.
+      + split. 1: auto.
+        eapply aux. auto.
+      + split. 1: auto.
+        eapply aux. auto.
     - eapply X17.
-      + eapply (All2_local_env_impl a). intros. apply X21.
-      + eapply (Hctx _ _ a), (All2_local_env_impl a). intros. apply (aux _ _ _ _ X21).
-      + eapply (All2_local_env_impl a0). intros. red. exact X21.
-      + eapply (All2_local_env_impl a0). intros. red. apply (aux _ _ _ _ X21).
-      + eapply (All2_All2_prop2_eq (Q:=P') (f:=dtype) (g:=dbody) a1 (extendP aux)).
-    - eapply (Hctx _ _ a), (All2_local_env_impl a). intros. apply (aux _ _ _ _ X21).
-    - eapply (All2_All2_prop (P:=pred1_extra) (Q:=P') a0 (extendP aux Γ Γ')).
-    - eapply (Hctx _ _ a), (All2_local_env_impl a). intros. apply (aux _ _ _ _ X21).
+      eapply All2_impl_def. 1: eauto.
+      intros [] []. cbn. intros [? [? ?]].
+      intuition auto.
+      + split. 1: auto.
+        eapply aux. auto.
+      + split. 1: auto.
+        eapply aux. auto.
+    - eapply All2_impl_def. 1: eauto.
+      intros.
+      split. 1: auto.
+      eapply aux. auto.
   Defined.
 
 End ParallelReductionExtra.
 
-Notation pred1_extra_ctx Σ e Γ Γ' :=
-  (All2_local_env (on_decl (pred1_extra Σ e)) Γ Γ').
+(* Notation pred1_extra_ctx Σ e Γ Γ' :=
+  (All2_local_env (on_decl (pred1_extra Σ e)) Γ Γ'). *)
 
-Lemma pred1_pred1_extra :
+(* Since we only have one context, it is not true
+  So we have to trust it's a good definition.
+  Examples will help see it is alright.
+*)
+(* Lemma pred1_pred1_extra :
   ∀ Σ Γ Δ u v e,
     pred1 Σ Γ Δ u v →
     pred1_extra Σ e Γ Δ u v.
@@ -533,51 +597,63 @@ Proof.
     eapply All2_impl. 1: eauto.
     intros ? ? [[? ?] [[? ?] ?]]. unfold on_Trel.
     intuition eauto.
-Qed.
+Qed. *)
 
 Lemma pred1_extra_pred1 :
   ∀ Σ Γ Δ u v e,
     on_Some (fun '(k, rd) =>
       lookup_env Σ k = Some (RewriteDecl rd)
     ) e →
-    pred1_extra Σ e Γ Δ u v →
+    pred1_extra Σ e Γ u v →
+    pred1_ctx Σ Γ Δ →
     pred1 Σ Γ Δ u v.
 Proof.
-  intros Σ Γ Δ u v e he h.
-  set (Pctx :=
-    fun Γ Δ =>
-      pred1_ctx Σ Γ Δ
-  ).
-  revert Γ Δ u v h.
-  refine (pred1_extra_ind_all_ctx Σ _ _ Pctx _ _ _ _ _ _ _ _ _ _ _ _ _ _ _ _ _ _ _ _ _ _ _ _ _ _).
-  all: try solve [ auto ].
+  intros Σ Γ Δ u v e he h hctx.
+  revert Γ u v h Δ hctx.
+  refine (pred1_extra_ind_all_ctx Σ _ _ _ _ _ _ _ _ _ _ _ _ _ _ _ _ _ _ _ _ _ _ _ _ _ _ _).
   all: try solve [ econstructor ; eauto ].
   all: try solve [
     intros ;
     econstructor ; eauto ;
     solve [ eapply All2_impl ; intuition eauto ; intuition eauto ]
   ].
+  all: try solve [
+    intros ;
+    econstructor ; eauto ;
+    try solve [ eapply All2_impl ; intuition eauto ; intuition eauto ] ;
+    match goal with
+    | h : ∀ Δ, pred1_ctx _ _ _ → pred1 _ _ _ ?u ?v |-
+      pred1 _ _ _ ?u ?v =>
+      eapply h
+    end ;
+    econstructor ; [
+      auto
+    | cbn ; eauto
+    ]
+  ].
   all: intros.
+  - econstructor. 1: auto.
+    (* NEED extra constructor for pred1 *)
+    give_up.
   - econstructor. all: eauto.
+    + induction X. 1: constructor.
+      (* HOW? *)
+      admit.
+    + admit.
     + eapply All2_impl. 1: eauto.
-      intros ? ? [? [[? ?] ?]]. intuition eauto.
-      unfold on_Trel in *. intuition eauto.
-    + eapply All2_impl. 1: eauto.
-      intros ? ? [? ?]. auto.
+      cbn. intuition auto.
   - econstructor. all: eauto.
+    + admit.
+    + admit.
     + eapply All2_impl. 1: eauto.
-      intros ? ? [[? ?] [[? ?] ?]]. unfold on_Trel.
-      intuition eauto.
+      cbn. intuition auto.
     + eapply All2_impl. 1: eauto.
-      intros ? ? [? ?]. auto.
-    + eapply All2_impl. 1: eauto.
-      intros ? ? [[? ?] ?]. intuition auto.
+      cbn. intuition auto.
   - econstructor. all: eauto.
+    + admit.
+    + admit.
     + eapply All2_impl. 1: eauto.
-      intros ? ? [[? ?] [[? ?] ?]]. unfold on_Trel.
-      intuition eauto.
-    + eapply All2_impl. 1: eauto.
-      intros ? ? [? ?]. auto.
+      cbn. intuition auto.
   - subst. cbn in he.
     match goal with
     | h : nth_error (all_rewrite_rules _) _ = _ |- _ =>
@@ -590,48 +666,29 @@ Proof.
     + eapply pred_rewrite_rule. all: eauto.
       eapply All2_impl. 1: eauto.
       intros ? ? [? ?]. auto.
-  - econstructor. all: eauto.
-    eapply All2_impl. 1: eauto.
-    intros ? ? [[? ?] [[? ?] ?]]. unfold on_Trel.
-    intuition eauto.
-  - econstructor. all: eauto.
-    eapply All2_impl. 1: eauto.
-    intros ? ? [[? ?] [[? ?] ?]]. unfold on_Trel.
-    intuition eauto.
-Qed.
+  - econstructor. 1: auto.
+    + admit.
+    + admit.
+  - econstructor. 1: auto.
+    + admit.
+    + admit.
+Admitted.
 
 Lemma weakening_env_pred1_extra :
-  ∀ `{cf : checker_flags} Σ Σ' e Γ Δ u v,
+  ∀ `{cf : checker_flags} Σ Σ' e Γ u v,
     wf Σ' →
     PCUICWeakeningEnv.extends Σ Σ' →
-    pred1_extra Σ e Γ Δ u v →
-    pred1_extra Σ' e Γ Δ u v.
+    pred1_extra Σ e Γ u v →
+    pred1_extra Σ' e Γ u v.
 Proof.
-  intros cf Σ Σ' e Γ Δ u v hΣ hx h.
-  set (Pctx :=
-    fun Γ Δ =>
-      pred1_extra_ctx Σ' e Γ Δ
-  ).
-  revert Γ Δ u v h.
-  refine (pred1_extra_ind_all_ctx Σ _ _ Pctx _ _ _ _ _ _ _ _ _ _ _ _ _ _ _ _ _ _ _ _ _ _ _ _ _ _).
-  all: try solve [ auto ].
+  intros cf Σ Σ' e Γ u v hΣ hx h.
+  revert Γ u v h.
+  refine (pred1_extra_ind_all_ctx Σ _ _ _ _ _ _ _ _ _ _ _ _ _ _ _ _ _ _ _ _ _ _ _ _ _ _ _).
   all: try solve [ econstructor ; eauto ].
   all: try solve [
     intros ;
     econstructor ; eauto ;
     solve [ eapply All2_impl ; intuition eauto ; intuition eauto ]
-  ].
-  all: try solve [
-    intros ;
-    unfold on_Trel in * ;
-    econstructor ; eauto ;
-    unfold on_Trel in * ;
-    solve [
-      eapply All2_impl ;
-      intuition eauto ;
-      unfold on_Trel in * ;
-      intuition eauto
-    ]
   ].
   - intros. eapply predx_rewrite_rule. all: eauto.
     + eapply PCUICWeakeningEnv.extends_lookup. all: eauto.
